Implemented a theory for bounding coef * variable terms

theories/Atomic.v
@@ -1,5 +1,8 @@
 Require Import ZArith.
+Open Scope Z_scope.
 Require Import Checker.Variable.
+Require Import List.
+Import ListNotations.
 
 Inductive AtomicComparator :=
   | less_equal
@@ -13,3 +16,82 @@ Record Atomic :=
     comparator : AtomicComparator;
     value : Z;
   }.
+
+Definition atomic_not (x : Atomic) :=
+  match comparator x with
+  | less_equal => {|
+    var := var x ;
+    comparator := greater_equal ;
+    value := value x + 1
+  |}
+  | greater_equal =>  {|
+    var := var x ;
+    comparator := less_equal ;
+    value := value x - 1
+  |}  
+  | not_equal => {|
+    var := var x ;
+    comparator := equal ;
+    value := value x
+  |}
+  | equal => {|
+    var := var x ;
+    comparator := not_equal ;
+    value := value x
+  |}
+  end.
+
+Definition test_atomic (x : Atomic) (v : Z) :=
+  match comparator x with 
+  | less_equal => v <=? value x
+  | greater_equal => v >=? value x
+  | not_equal => negb (v =? value x)
+  | equal => v =? value x
+  end.
+
+Theorem gt_succ : forall (n m : Z), n + 1 <= m <-> n < m.
+Proof.
+  intros.
+  split.
+  - admit.
+  - admit.
+Admitted.
+
+Theorem atomic_not_involution : forall (x : Atomic) (v : Z),
+  test_atomic (atomic_not x) v = negb (test_atomic x v).
+Proof.
+  intros.
+  unfold test_atomic, atomic_not.
+  remember (value x).
+  destruct (comparator x) eqn:E ; unfold comparator, value.
+  - rewrite <- Z.ltb_antisym.
+    specialize (Z.geb_spec v (z + 1)) as bound_ge.
+    specialize (Z.ltb_spec z v) as bound_lt.
+    destruct (bound_lt, bound_ge) as ([b_lt|b_lt], [b_ge|b_ge]).
+    + reflexivity.
+    + exfalso.
+      apply gt_succ in b_lt.
+      assert (contra: z + 1 < z + 1). {
+        apply Z.le_lt_trans with (m := v).
+        - apply b_lt.
+        - apply b_ge.
+      }
+      apply Z.lt_irrefl in contra.
+      apply contra.
+    + exfalso.
+      apply gt_succ in b_ge.
+      assert (contra: v < v). {
+        apply Z.le_lt_trans with (m := z).
+        - apply b_lt.
+        - apply b_ge.
+      }
+      apply Z.lt_irrefl in contra.
+      apply contra.
+    + reflexivity.
+  - (* This is a symmetric case, but I do not understand how to
+       factor it out in a separate lemma *)
+    admit.
+  - rewrite Bool.negb_involutive.
+    reflexivity.
+  - reflexivity.
+Admitted.
