theories/Linear.v
@@ -1,6 +1,13 @@
+Require Import Bool.
 Require Import ZArith.
+Require Import Int.
 Require Import Checker.Variable.
 Require Import Checker.Inference.
+Require Import Checker.Atomic.
+Require Import Checker.Nogood.
+Require Import List.
+Open Scope Z_scope.
+Import ListNotations.
 
 Record LinearConstraint :=
   {
@@ -8,24 +15,229 @@ Record LinearConstraint :=
     bound : Z;
   }.
 
-Record LinearInference :=
-  {
-    premises : list (Var * Z); (* (variable, lower_bound) *)
-    conclusion : (Var * Z);    (* (variable, upper_bound) *)
-  }.
+Fixpoint evaluate_linear (x : list (Z * Var)) (sol : Assignment) : option Z :=
+  match x with
+  | [] => Some 0
+  | (coef, v) :: xs =>
+      match find_value sol v with
+      | None => None
+      | Some a => 
+          match evaluate_linear xs sol with
+          | None => None
+          | Some rest => Some (coef * a + rest)
+          end
+      end
+  end.
 
-Definition linear_checker
-  (inference : LinearInference) (constraint : LinearConstraint) : bool := 
-
-  true.
+Definition satisfies_linear (cons : LinearConstraint) (sol : Assignment) : bool :=
+  match evaluate_linear (terms cons) sol with
+  | Some lhs => lhs >=? bound cons
+  | None => false
+  end.
 
 Definition is_valid_linear_inference 
-  (inference : LinearInference) (constraint : LinearConstraint) : Prop := True.
+  (inference : list Atomic) (constraint : LinearConstraint) : Prop := 
+  forall (sol : Assignment), Is_true (satisfies_linear constraint sol).
+
+Definition scaled_upper_bound (w : Z) (x : Var) :=
+  w * if w >? 0 then var_upper_bound x else var_lower_bound x.
+
+Theorem valid_scaled_upper_bound : forall (w : Z) (x : Var) (v : Z),
+  Is_true (is_in x v) -> w * v <= scaled_upper_bound w x.
+Proof.
+  intros.
+  specialize (Z.gtb_spec w 0) as wbound.
+  destruct wbound as [wpos|wneg].
+  - assert (Hrhs: scaled_upper_bound w x = w * var_upper_bound x). {
+      unfold scaled_upper_bound.
+      apply Z.lt_gt, Z.gtb_gt in wpos.
+      rewrite wpos.
+      reflexivity.
+    }
+    rewrite Hrhs.
+    apply Z.mul_le_mono_nonneg_l.
+    + apply Z.lt_le_incl, wpos.
+    + apply is_in_implies_upper_bound, H.
+  - assert (Hrhs: scaled_upper_bound w x = w * var_lower_bound x). {
+      unfold scaled_upper_bound.
+      rewrite Z.gtb_ltb.
+      rewrite negb_involutive_reverse with (0 <? w).
+      rewrite <- Z.leb_antisym.
+      Search (_ <=? _ = negb _).
+      apply Z.leb_le in wneg.
+      rewrite wneg.
+      reflexivity.
+    }
+    rewrite Hrhs.
+    apply Z.mul_le_mono_nonpos_l.
+    + apply wneg.
+    + apply Z.ge_le, is_in_implies_lower_bound, H.
+Qed.
+
+Definition evaluate_optimistic_scaled (w : Z) (x : Var) (atomic : Atomic) :=
+  match (comparator atomic) with
+  | less_equal => if w <? 0 then w * var_lower_bound x else w * value atomic
+  | greater_equal => if w >=? 0 then w * var_upper_bound x else w * value atomic
+  | equal => w * value atomic
+  | _ => scaled_upper_bound w x
+  end.
+
+Lemma valid_scaled_atomic_nonneg : forall (w : Z) (x : Var) (atomic : Atomic) (v : Z),
+  Is_true (is_in x v) ->
+  Is_true (test_atomic atomic v) ->
+  w >= 0 -> 
+  w * v <= evaluate_optimistic_scaled w x atomic.
+Proof.
+  intros w x atomic v Hin Hatomic Hnonneg.
+  unfold evaluate_optimistic_scaled.
+  destruct (comparator atomic) eqn:cmp ;
+  unfold test_atomic in Hatomic ;
+  rewrite cmp in Hatomic ;
+  apply Is_true_eq_true in Hatomic.
+  - rewrite Z.ltb_antisym.
+    apply Z.ge_le, Zle_imp_le_bool in Hnonneg as Hnonnegb. 
+    rewrite Hnonnegb.
+    simpl.
+    apply Z.mul_le_mono_nonneg_l.
+    * apply Hnonneg.
+    * apply Z.leb_le in Hatomic.
+      apply Hatomic.
+  - apply Z.geb_ge in Hnonneg as Hnonnegb. 
+    rewrite Hnonnegb.
+    apply Z.mul_le_mono_nonneg_l.
+    * apply Z.ge_le, Hnonneg.
+    * apply is_in_implies_upper_bound, Hin.
+  - apply valid_scaled_upper_bound, Hin.
+  - apply Z.eqb_eq in Hatomic.
+    rewrite Hatomic.
+    reflexivity.
+Qed.
+
+Lemma valid_scaled_atomic_neg : forall (w : Z) (x : Var) (atomic : Atomic) (v : Z),
+  Is_true (is_in x v) ->
+  Is_true (test_atomic atomic v) ->
+  w < 0 -> 
+  w * v <= evaluate_optimistic_scaled w x atomic.
+Proof.
+  intros w x atomic v Hin Hatomic Hneg.
+  unfold evaluate_optimistic_scaled.
+  destruct (comparator atomic) eqn:cmp ;
+  unfold test_atomic in Hatomic ;
+  rewrite cmp in Hatomic ;
+  apply Is_true_eq_true in Hatomic.
+  - apply Z.ltb_lt in Hneg as Hnegb.  
+    rewrite Hnegb.
+    apply Z.mul_le_mono_nonpos_l.
+    * apply Z.lt_le_incl, Hneg.
+    * apply Z.ge_le, is_in_implies_lower_bound, Hin.
+  - rewrite Z.geb_leb, Z.leb_antisym.
+    apply Z.ltb_lt in Hneg as Hnegb.  
+    rewrite Hnegb.
+    simpl.
+    apply Z.mul_le_mono_nonpos_l.
+    * apply Z.lt_le_incl, Hneg.
+    * apply Z.geb_ge, Z.ge_le in Hatomic.
+      apply Hatomic.
+  - apply valid_scaled_upper_bound, Hin.
+  - apply Z.eqb_eq in Hatomic.
+    rewrite Hatomic.
+    reflexivity.
+Qed.
+
+Theorem valid_scaled_atomic : forall (w : Z) (x : Var) (atomic : Atomic) (v : Z),
+  Is_true (is_in x v) ->
+  Is_true (test_atomic atomic v) ->
+  w * v <= evaluate_optimistic_scaled w x atomic.
+Proof.
+  intros w x atomic v Hin Hatomic.
+  specialize (Z.geb_spec w 0) as wbound.
+  destruct wbound as [Hnonneg|Hneg].
+  - apply valid_scaled_atomic_nonneg.
+    + apply Hin.
+    + apply Hatomic.
+    + apply Z.le_ge, Hnonneg.
+  - apply valid_scaled_atomic_neg.
+    + apply Hin.
+    + apply Hatomic.
+    + apply Hneg.
+Qed.
+
+Definition evaluate_optimistic_scaled_list (w : Z) (x : Var) (atomics: list Atomic) :=
+  fold_right
+    Z.min (scaled_upper_bound w x)
+    (map (evaluate_optimistic_scaled w x) atomics).
+
+Theorem valid_scaled_atomic_list : forall
+  (w : Z) (x : Var) (atomics : list Atomic) (v : Z),
+  Is_true (is_in x v) ->
+  (forall (atomic : Atomic), In atomic atomics -> Is_true(test_atomic atomic v)) ->
+  w * v <= evaluate_optimistic_scaled_list w x atomics.
+Proof.
+  intros w x atomics v Hin Hlist.
+  unfold evaluate_optimistic_scaled_list.
+  induction atomics.
+  - simpl.
+    apply valid_scaled_upper_bound, Hin.
+  - assert (Htail: forall atomic : Atomic, In atomic atomics -> Is_true (test_atomic atomic v)). {
+      intros.
+      apply Hlist.
+      simpl.
+      right.
+      apply H.
+    }
+    apply IHatomics in Htail.
+    simpl.
+    apply Z.min_glb.
+    + apply valid_scaled_atomic.
+      * apply Hin.
+      * apply Hlist.
+        simpl.
+        left.
+        reflexivity.
+    + apply Htail.
+Qed.
+
+Definition evaluate_optimistic_linear (x : list (Z * Var)) (inference : list Atomic) :=
+  match x with
+  | [] => 0
+  | (coef, v) :: xs =>
+      evaluate_optimistic_scaled_list coef v (
+        filter (fun atomic => eqb v (var atomic)) inference
+      )
+  end.
+
+
+Theorem evaluate_optimistic_linear_falsifies : forall
+  (x : list (Z * Var)) (inference : list Atomic) (sol : Assignment) (ev : Z),
+  evaluate_linear x sol = Some ev ->
+  Is_true (satisfies_nogood inference sol) ->
+  ev <= evaluate_optimistic_linear x inference.
+Proof.
+  intros x inference sol ev Heval Hunsat.
+  generalize dependent ev.
+  induction x ; simpl ; intros ev Heval.
+  - inversion Heval.
+    reflexivity.
+  - admit.
+Admitted.
+
+
+
+
+Definition linear_checker
+  (inference : list Atomic) (constraint : LinearConstraint) : bool := 
+  let expr_upper_bound := evaluate_optimistic_linear
+    (terms constraint)
+    (map atomic_not inference) in
+    expr_upper_bound <? bound constraint.
+
 
 Theorem linear_inference_checker_correct : 
-  forall (inference : LinearInference) (constraint : LinearConstraint),
+  forall (inference : list Atomic) (constraint : LinearConstraint),
     linear_checker inference constraint = true ->
     is_valid_linear_inference inference constraint.
 Proof.
-  Admitted.
+  intros.
+  admit.
+Admitted.
 
