theories/Variable.v
@@ -1,3 +1,4 @@
+Require Import Bool.
 Require Import List.
 Require Import String.
 Require Import ZArith.
@@ -12,8 +13,75 @@ Record IntervalVariable :=
     upper_bound : Z := lower_bound + Z.of_nat (proj1_sig size)
   }.
 
+Compute upper_bound {| name := "a"; lower_bound := 1; size := exist _ 5 (Nat.neq_succ_0 4) |}.
+
+Open Scope Z_scope.
+
 Inductive Var :=
   | interval (var : IntervalVariable).
 
-Compute upper_bound {| name := "a"; lower_bound := 1; size := exist _ 5 (Nat.neq_succ_0 4) |}.
+Definition eqb (lhs : Var) (rhs : Var) :=
+  match (lhs, rhs) with
+  | (interval lhs, interval rhs) => String.eqb (name lhs) (name rhs)
+  end.
+
+Definition var_lower_bound (x : Var) :=
+  match x with
+  | interval val => lower_bound val
+  end.
+
+Definition var_upper_bound (x : Var) :=
+  match x with
+  | interval val => upper_bound val
+  end.
+
+Definition is_in (x : Var) (val : Z) :=
+  match x with
+  | interval var => andb (lower_bound var <=? val) (val <=? upper_bound var)
+  end.
+
+Theorem is_in_implies_lower_bound : forall (x : Var) (val : Z),
+  Is_true (is_in x val) -> val >= var_lower_bound x.
+Proof.
+  intros.
+  destruct x.
+  simpl.
+  unfold is_in in H.
+  apply andb_prop_elim in H.
+  destruct H as [Hlb].
+  apply Is_true_eq_true, Z.leb_le, Z.le_ge in Hlb.
+  apply Hlb.
+Qed.
+
+Theorem is_in_implies_upper_bound : forall (x : Var) (val : Z),
+  Is_true (is_in x val) -> val <= var_upper_bound x.
+Proof.
+  intros.
+  destruct x.
+  simpl.
+  unfold is_in in H.
+  apply andb_prop_elim in H.
+  destruct H as [_ Hub].
+  apply Is_true_eq_true, Z.leb_le in Hub.
+  apply Hub.
+Qed.
+
+Record VariableAssignment := {
+  variable : Var ;
+  assigned : Z
+}.
+
+Definition consistent (x : VariableAssignment) := is_in (variable x) (assigned x).
+
+Record Assignment := {
+  mapping : list VariableAssignment ;
+  consistency_prop : Is_true (forallb consistent mapping)
+}.
+
+Definition find_value (sol : Assignment) (var : Var) :=
+  match find (fun x => eqb (variable x) var) (mapping sol) with
+  | Some a => Some (assigned a)
+  | None => None
+  end.
+
 
