theories/ConstraintProblem.v
@@ -1,6 +1,10 @@
 Require Import Checker.Variable.
 Require Import Checker.Atomic.
 Require Import Checker.Linear.
+Require Import Checker.Nogood.
+Require Import ZArith.
+Require Import List.
+Open Scope Z_scope.
 
 Inductive Constraint :=
   | linear_leq (constraint : LinearConstraint)
@@ -12,3 +16,8 @@ Record ConstraintProblem :=
     constraints : list Constraint;
   }.
 
+Definition satisfies_constraint (c : Constraint) (sol : list Assignment) :=
+  match c with
+  | linear_leq lin => satisfies_linear lin sol
+  | nogood atomics => satisfies_nogood atomics sol
+  end.
