theories/Nogood.v
@@ -1,0 +1,17 @@
+Require Import Checker.Variable.
+Require Import Checker.Atomic.
+Require Import ZArith.
+Require Import List.
+Open Scope Z_scope.
+
+Fixpoint satisfies_nogood (x : list Atomic) (sol : Assignment) :=
+  match x with
+  | nil => false
+  | a :: xs =>
+      let maybe_value := find_value sol (var a) in
+      match maybe_value with
+      | Some v => if test_atomic a v then true else satisfies_nogood xs sol
+      | None => false
+      end
+  end.
+
